add Conf and helper functions

theories/opsem/basic.v
@@ -1,6 +1,6 @@
 From Coq Require Import Eqdep_dec.
 From Coq.micromega Require Import ZifyClasses.
-From stdpp Require Import gmap fin_maps list.
+From stdpp Require Import base gmap fin_maps list.
 
 
 
@@ -106,6 +106,10 @@ Definition WordNum : Z :=Z.pow 2 64.
 Inductive Word: Type :=
 | W (z : Z) (fin: Z.leb z WordNum = true) (pos: Z.leb 0 z = true).
 
+Definition z_of_w (w: Word): Z :=
+  match w with
+  | W z _ _ => z
+  end.
 
 Definition GenReg := gmap GenRegName Word.
 Definition SysReg := gmap SysRegName Word.
@@ -116,7 +120,6 @@ Proof.
   - exact w.
   - exact (W WordNum eq_refl eq_refl).
 Defined.
-
 Definition SysRegLocate (reg : SysReg) (r : SysRegName) : Word.
 Proof.
   destruct (reg !! r).
@@ -160,15 +163,15 @@ Definition MemNum : Z := Z.pow 2 48.
 Inductive Addr: Type :=
 | A (z : Z) (fin: Z.leb z MemNum = true) (pos: Z.leb 0 z = true).
 
-Definition z_of (a: Addr): Z :=
+Definition z_of_a (a: Addr): Z :=
   match a with
   | A z _ _ => z
   end.
 
-Coercion z_of: Addr >-> Z.
+Coercion z_of_a: Addr >-> Z.
 
 Lemma z_of_eq a1 a2 :
-  z_of a1 = z_of a2 ->
+  z_of_a a1 = z_of_a a2 ->
   a1 = a2.
 Proof.
   destruct a1, a2; cbn. intros ->.
@@ -177,7 +180,7 @@ Qed.
 
 Lemma eq_z_of a1 a2 :
   a1 = a2 ->
-  z_of a1 = z_of a2.
+  z_of_a a1 = z_of_a a2.
 Proof. destruct a1; destruct a2. congruence. Qed.
 
 Global Instance addr_eq_dec: EqDecision Addr.
@@ -187,22 +190,27 @@ intros x y. destruct x,y. destruct (Z_eq_dec z z0).
 - right. inversion 1. simplify_eq.
 Defined.
 
-Definition z_to_addr (z : Z) : option Addr.
+Definition z_to_addr (z : Z) :  Addr.
 Proof.
   destruct (Z_le_dec z MemNum),(Z_le_dec 0 z).
   - apply (Z.leb_le z MemNum) in l.
     apply (Z.leb_le 0 z) in l0.
-    exact (Some (A z l l0)).
-  - exact None.
-  - exact None.
-  - exact None.
+    exact (A z l l0).
+  - exact (A MemNum eq_refl eq_refl).
+  - exact (A 0 eq_refl eq_refl).
+  - apply (Znot_le_gt _ _) in n.
+    exfalso.
+    apply n0.
+    assert (0< z)%Z.
+    { apply (Z.lt_trans _ MemNum _). done. apply Z.gt_lt in n. assumption. }
+    lia.
 Defined.
 
 Global Instance addr_countable : Countable Addr.
 Proof.
-  refine {| encode r := encode (z_of r) ;
+  refine {| encode r := encode (z_of_a r) ;
             decode n := match (decode n) with
-                        | Some z => z_to_addr z
+                        | Some z => Some (z_to_addr z)
                         | None => None
                         end ;
             decode_encode := _ |}.
@@ -385,7 +393,7 @@ Proof.
       done.
 Defined.
 
-Definition pid_of (a : Addr) : PID.
+Definition a_to_pid (a : Addr) : PID.
 Proof.
   destruct a.
   assert(z ≫ PageBitSize ≤ PIDNum)%Z.
@@ -408,16 +416,312 @@ Defined.
 Definition VMID :Type := nat.
 
 
-(*TODO: MailBox*)
+(*MailBox*)
 
+Definition MB :Type := (option PID) * option(PID * bool * Word * VMID).
 
 
 (*TODO: State*)
 
+Definition z_of_p (p: PID): Z :=
+  match p with
+  | P z _ _ => z
+  end.
+
+Coercion z_of_p: PID >-> Z.
+
+Lemma z_of_p_eq a1 a2 :
+  z_of_p a1 = z_of_p a2 ->
+  a1 = a2.
+Proof.
+  destruct a1, a2; cbn. intros ->.
+  repeat f_equal; apply eq_proofs_unicity; decide equality.
+Qed.
+
+Lemma eq_z_of_p a1 a2 :
+  a1 = a2 ->
+  z_of_p a1 = z_of_p a2.
+Proof. destruct a1; destruct a2. congruence. Qed.
 
 
-(*TODO: ShareState*)
+Global Instance pid_eq_dec: EqDecision PID.
+Proof.
+intros x y. destruct x,y. destruct (Z_eq_dec z z0).
+- left. subst z0. eapply z_of_p_eq; eauto.
+- right. inversion 1. simplify_eq.
+Defined.
+
+Definition z_to_pid (z : Z) : PID.
+Proof.
+  destruct (Z_le_dec z PIDNum),(Z_le_dec 0 z).
+  - apply (Z.leb_le z PIDNum) in l.
+    apply (Z.leb_le 0 z) in l0.
+    exact (P z l l0).
+  - exact (P PIDNum eq_refl eq_refl).
+  - exact (P 0 eq_refl eq_refl).
+  - apply (Znot_le_gt _ _) in n.
+    exfalso.
+    apply n0.
+    assert (0< z)%Z.
+    { apply (Z.lt_trans _ PIDNum _). done. apply Z.gt_lt in n. assumption. }
+    lia.
+Defined.
+
+
+Global Instance pid_countable : Countable PID.
+Proof.
+  refine {| encode r := encode (z_of_p r) ;
+            decode n := match (decode n) with
+                        | Some z => Some (z_to_pid z)
+                        | None => None
+                        end ;
+            decode_encode := _ |}.
+  intro r. destruct r; auto.
+  rewrite decode_encode.
+  unfold z_to_pid. simpl.
+  destruct (Z_le_dec z PIDNum),(Z_le_dec 0 z).
+  - repeat f_equal; apply eq_proofs_unicity; decide equality.
+  - exfalso. by apply (Z.leb_le 0 z) in pos.
+  - exfalso. by apply (Z.leb_le z PIDNum) in fin.
+  - exfalso. by apply (Z.leb_le z PIDNum) in fin.
+Defined.
+
+Definition State: Type := (gset PID) *( GenReg * (SysReg * MB)).
+
+
+(*ShareState*)
+
+Definition ShareStates: Type := list (PID * VMID).
+
+
+(*ExecConf*)
+
+Definition ExecConf: Type := list State * (Mem * ShareStates).
+
+
+(*ExecMode*)
+
+Inductive DoneState: Type:=
+| Next (v: VMID)
+| Halt
+| Fail.
+
+Inductive ExecMode: Type :=
+| ExecInstr (v: VMID)
+| Repeat (u : ExecMode)
+| Done (d : DoneState).
+
+
+(*Conf*)
+
+Definition Conf : Type := ExecMode * ExecConf.
+
+Implicit Type ϕ : ExecConf.
+Implicit Type Δ : list (State).
+Implicit Type δ : State.
+Implicit Type m : Mem.
+Implicit Type s : ShareStates.
+Implicit Type v n : VMID.
+
+Definition mem_of  ϕ  : Mem := fst (snd ϕ) .
+
+Fixpoint ith_of {A} (l: list A) (i:nat): option A :=
+  match i with
+  | 0 => match l with
+         | cons a _ => Some a
+         |  nil => None
+         end
+  | S n => match l with
+           |  nil => None
+           |  cons a l' => ith_of l' n
+           end
+  end.
+
+
+Definition state_of Δ (v:VMID) : option State := ith_of Δ v.
+
+Definition sysreg_of δ: SysReg := fst (snd (snd δ)).
+
+Definition genreg_of δ: GenReg := fst (snd δ).
+
+Definition pids_of δ : gset PID := fst δ.
+
+Definition mb_of δ : MB := snd (snd (snd δ)).
+
+Notation "ϕ .m" := (mem_of ϕ) (at level 20).
+Notation "δ .gr" := (genreg_of δ) (at level 20).
+Notation "δ .sr" := (sysreg_of δ) (at level 20).
+Notation "δ .ps" := (pids_of δ) (at level 20).
+Notation "δ .π" := (mb_of δ) (at level 20).
+Notation "Δ !s! i " := (state_of Δ i) (at level 20).
+Notation "g !gr! r " := (GenRegLocate g r)(at level 20).
+Notation "s !sr! r " := (SysRegLocate s r)(at level 20).
+
+
+Inductive MemPermission :Type :=
+| VA
+| RE
+| WR.
+
+
+(* helper functions *)
+Definition w_to_a (w:Word): Addr.
+Proof.
+  destruct w.
+  destruct (Z_le_dec z MemNum).
+  - apply (Z.leb_le z MemNum) in l.
+    exact (A z l pos).
+  - exact (A MemNum eq_refl eq_refl).
+Defined.
+
+Definition valid_a δ (r: GenRegName) (p : MemPermission) : option Addr.
+Proof.
+  destruct p eqn:Hp.
+  - exact ((gset_to_gmap (w_to_a (δ.gr !gr! r)) (pids_of δ)) !! (a_to_pid (w_to_a (δ.gr !gr! r)))).
+  - destruct (δ.π.2).
+    + destruct p0.1.1.
+      destruct (decide ((a_to_pid (w_to_a (δ.gr !gr! r)))=p1)).
+      exact (Some (w_to_a (δ.gr !gr! r))).
+      exact ((gset_to_gmap (w_to_a (δ.gr !gr! r)) (pids_of δ)) !! (a_to_pid (w_to_a (δ.gr !gr! r)))).
+    + exact ((gset_to_gmap (w_to_a (δ.gr !gr! r)) (pids_of δ)) !! (a_to_pid (w_to_a (δ.gr !gr! r)))).
+  - destruct (δ.π.1).
+    + destruct (decide ((a_to_pid (w_to_a (δ.gr !gr! r)))=p0)).
+      exact (Some (w_to_a (δ.gr !gr! r))).
+      exact ((gset_to_gmap (w_to_a (δ.gr !gr! r)) (pids_of δ)) !! (a_to_pid (w_to_a (δ.gr !gr! r)))).
+    + exact ((gset_to_gmap (w_to_a (δ.gr !gr! r)) (pids_of δ)) !! (a_to_pid (w_to_a (δ.gr !gr! r)))).
+Defined.
+
+Definition w_add_z (w: Word) (i:Z) : Word.
+Proof.
+  destruct w.
+  assert ((0 ≤ (Z.modulo (z+i) WordNum) )%Z
+          ∧ ((Z.modulo (z+i) WordNum)< WordNum)%Z).
+  { apply (Z_mod_lt (z+i) WordNum). done. }
+  destruct H.
+  apply (Z.leb_le 0 (Z.modulo (z+i) WordNum)) in H.
+  apply Z.lt_le_incl in H0.
+  apply (Z.leb_le (Z.modulo (z+i) WordNum) WordNum) in H0.
+  exact (W (Z.modulo (z+i) WordNum) H0 H).
+Defined.
+
+Definition w_add_w (w1: Word) (w2: Word) : Word:=
+  match w2 with
+  | W z _ _ => (w_add_z w1 z)
+  end.
+
+Definition w_sub_z (w: Word) (i:Z) : Word.
+Proof.
+  destruct w.
+  assert ((0 ≤ (Z.modulo (z-i) WordNum) )%Z
+          ∧ ((Z.modulo (z-i) WordNum)< WordNum)%Z).
+  { apply (Z_mod_lt (z-i) WordNum). done. }
+  destruct H.
+  apply (Z.leb_le 0 (Z.modulo (z-i) WordNum)) in H.
+  apply Z.lt_le_incl in H0.
+  apply (Z.leb_le (Z.modulo (z-i) WordNum) WordNum) in H0.
+  exact (W (Z.modulo (z-i) WordNum) H0 H).
+Defined.
+
+Definition w_sub_w (w1: Word) (w2: Word) : Word:=
+  match w2 with
+  | W z _ _ => (w_sub_z w1 z)
+  end.
+
+
+Definition upd_gen_reg Δ v (r: GenRegName) (w: Word): list State :=
+  match (Δ !s! v) with
+    | Some δ => <[v:=(δ.ps, (<[r:=w]>(δ.gr), (δ.sr, δ.π )))]>Δ
+    | None => Δ
+  end.
+
+Definition upd_sys_reg Δ v (r: SysRegName) (w: Word): list State :=
+  match (Δ !s! v) with
+    | Some δ => <[v:=(δ.ps, ( δ.gr ,(<[r:=w]>(δ.sr), δ.π )))]>Δ
+    | None => Δ
+  end.
 
 
 
-(*TODO: ExecConf*)
+Definition updPC Δ m s v: ExecConf :=
+  match (Δ !s! v) with
+  |Some δ => ((upd_gen_reg Δ v PC (w_add_z ((δ.gr) !gr! PC) 1)) ,(m,s))
+  |None => (Δ, (m,s))
+  end.
+
+Definition ident Δ m s v: ExecConf :=
+  (Δ, (m,s)).
+
+Inductive ReturnCode: Type:=
+|INTERRUPT
+|SUCCESS
+|BUSY
+|MSG_WAIT
+|MSG_SEND
+|MEM_RTRVP
+|YIELD.
+
+Definition rc_to_w (rc : ReturnCode):Word.
+Proof.
+  destruct rc eqn:Hrc.
+  - exact (W 0 eq_refl eq_refl).
+  - exact (W 1 eq_refl eq_refl).
+  - exact (W 2 eq_refl eq_refl).
+  - exact (W 3 eq_refl eq_refl).
+  - exact (W 4 eq_refl eq_refl).
+  - exact (W 5 eq_refl eq_refl).
+  - exact (W 6 eq_refl eq_refl).
+Defined.
+
+Definition z_to_w (z:Z):Word.
+Proof.
+  destruct (Z_le_dec 0%Z z), (Z_le_dec z WordNum).
+  - apply (Z.leb_le 0 z) in l.
+    apply (Z.leb_le z WordNum) in l0.
+    exact (W z l0 l).
+  - exact (W WordNum eq_refl eq_refl).
+  - exact (W 0 eq_refl eq_refl).
+  - apply (Znot_le_gt _ _) in n0.
+    exfalso.
+    apply n.
+    assert (0< z)%Z.
+    { apply (Z.lt_trans _ WordNum _). done. apply Z.gt_lt in n0. assumption. }
+    lia.
+Defined.
+
+
+Definition nat_to_w (n:nat):Word:=
+(z_to_w (Z.of_nat n)).
+
+Definition nat_to_r (n:nat):GenRegName.
+Proof.
+  destruct (decide(n≤ RegNum)).
+  - apply (Nat.leb_le n RegNum) in l.
+    exact (R n l).
+  - exact (R RegNum eq_refl).
+Defined.
+
+Definition tick Δ m s v n (f: list State -> Mem -> ShareStates -> VMID -> ExecConf): Conf :=
+  match (Δ !s! 0) with
+  | Some δ_p =>match (Δ !s! v) with
+                 | Some δ_v =>if (andb (Z.leb (z_of_w (δ_p.sr !sr! CNTVAL)) 1) (Z.eqb (z_of_w (δ_p.sr !sr! CNTCTL)) 1)) then
+                                let Δ' := upd_sys_reg Δ 0 CNTVAL (w_sub_z (δ_p.sr !sr! CNTVAL) 1) in
+                                let Δ' := upd_sys_reg Δ' 0 CNTCTL (z_to_w 0) in
+                                let Δ' := upd_gen_reg Δ' 0 (nat_to_r 0) (rc_to_w INTERRUPT) in
+                                let Δ' := upd_gen_reg Δ' 0 (nat_to_r 1) (nat_to_w v) in
+                                ((Done (Next 0)),(f Δ' m s v))
+                              else
+                                let Δ' := upd_sys_reg Δ 0 CNTVAL (w_sub_z (δ_p.sr !sr! CNTVAL) 1) in
+                                ((Done (Next n)),(f Δ' m s v))
+                 |None => (Done Fail, (Δ,(m, s)))
+               end
+  |None => (Done Fail, (Δ, (m, s )))
+  end.
+
+
+Definition comb (w1 w2 : Word) : Word:=
+  match w1 with
+  | (W z _ _) => w_add_z w2 (Z.shiftl z 32)
+  end.
+
+
+(*TODO decode*)
